src/tactic/aesop/tracing.lean
@@ -4,11 +4,11 @@ Released under Apache 2.0 license as described in the file LICENSE.
 Authors: Jannis Limperg
 -/
 
-import tactic.auto.tree
+import tactic.aesop.tree
 
-declare_trace auto.steps
-declare_trace auto.tree
-declare_trace auto.rule_set
+declare_trace aesop.steps
+declare_trace aesop.tree
+declare_trace aesop.rule_set
 
 variables {α β : Type} [has_to_tactic_format α] [has_to_tactic_format β]
 
@@ -21,22 +21,22 @@ meta def trace_nested (n : name) (tag : string) (header : α) (body : β) :
   tactic unit :=
 when_tracing n $ trace! "[{tag}] {header}{format.nested 2 <$> pp body}"
 
-namespace auto
+namespace aesop
 
 meta def trace : α → tactic unit :=
-trace_tagged `auto.steps "auto"
+trace_tagged `aesop.steps "aesop"
 
 meta def trace_nested : α → β → tactic unit :=
-tactic.trace_nested `auto.steps "auto"
+tactic.trace_nested `aesop.steps "aesop"
 
 meta def trace_separator : tactic unit :=
 trace "================================================================================"
 
 meta def trace_tree (t : tree) : tactic unit :=
-tactic.trace_nested `auto.tree "auto" "search tree" t
+tactic.trace_nested `aesop.tree "aesop" "search tree" t
 
 meta def trace_rule_set (rs : rule_set) : tactic unit :=
-tactic.trace_nested `auto.rule_set "auto" "rule set" rs
+tactic.trace_nested `aesop.rule_set "aesop" "rule set" rs
 
-end auto
+end aesop
 end tactic
